CBPV/ClosedSemantics.lean
@@ -1,7 +1,7 @@
 import CBPV.Evaluation
 import CBPV.Typing
 
-open ValType ComType Val Com
+open Nat ValType ComType Val Com
 
 /-*--------------------------
   Logical relation on types
@@ -58,21 +58,35 @@ theorem 𝒞bwd {B m n} (r : m ⇒⋆ n) (h : n ∈ ⟦ B ⟧ᶜ) : m ∈ ⟦ B 
   Semantic typing
 ----------------*-/
 
--- Semantic well-formedness of contexts
 def semCtxt Γ (σ : Nat → Val) := ∀ {x A}, Γ ∋ x ∶ A → σ x ∈ ⟦ A ⟧ᵛ
 notation:40 Γ:41 "⊨" σ:41 => semCtxt Γ σ
 
--- Convenient constructors for semantic contexts
 theorem semCtxtNil : ⬝ ⊨ var := by intro _ _ mem; cases mem
 theorem semCtxtCons {Γ σ v A} (h : v ∈ ⟦ A ⟧ᵛ) (hσ : Γ ⊨ σ) : Γ ∷ A ⊨ v +: σ
   | _, _, .here => h
   | _, _, .there mem => hσ mem
 
+def semDtxt Γ Δ (τ : Nat → Com) := ∀ {σ j v A B}, Γ ⊨ σ → Δ ∋ j ∶ A ↗ B → v ∈ ⟦ A ⟧ᵛ → (τ j)⦃v +: σ⦄ ∈ ⟦ B ⟧ᵉ
+notation:40 Γ:41 "∣" Δ:41 "⊨" τ:41 => semDtxt Γ Δ τ
+
+theorem semDtxtNil {Γ} {τ : Nat → Com} : Γ ∣ ⬝ ⊨ τ := λ _ mem ↦ by cases mem
+
+theorem semDtxtCons₁ {Γ Δ τ A} (hτ : Γ ∣ Δ ⊨ τ) : Γ ∷ A ∣ Δ ⊨ renameCom (lift succ) ∘ τ := by
+  intro σ j v _ _ hσ mem; simp
+  rw [substRenameCom, substComExt _ (v +: σ ∘ succ) (λ n ↦ ?e)]
+  case e => cases n <;> simp [lift]
+  exact hτ (λ mem ↦ hσ (.there mem)) mem
+
+theorem semDtxtCons₂ {Γ Δ τ m A B} (h : ∀ {σ v}, Γ ⊨ σ → v ∈ ⟦ A ⟧ᵛ → m⦃v +: σ⦄ ∈ ⟦ B ⟧ᵉ) (hτ : Γ ∣ Δ ⊨ τ) : Γ ∣ Δ ∷ A ↗ B ⊨ m +: τ := by
+  intro _ _ _ _ _ hσ mem; cases mem
+  case here => exact h hσ
+  case there mem => exact hτ hσ mem
+
 -- Semantic typing of values and computations
-@[simp] def semVal Γ v A := ∀ σ, Γ ⊨ σ → v⦃σ⦄ ∈ ⟦ A ⟧ᵛ
-@[simp] def semCom Γ m B := ∀ σ, Γ ⊨ σ → m⦃σ⦄ ∈ ⟦ B ⟧ᵉ
+@[simp] def semVal (Γ : Ctxt) v A := ∀ σ, Γ ⊨ σ → v⦃σ⦄ ∈ ⟦ A ⟧ᵛ
+@[simp] def semCom (Γ : Ctxt) (Δ : Dtxt) m B := ∀ σ, Γ ⊨ σ → ∀ τ, Γ ∣ Δ ⊨ τ → (substJoin τ m)⦃σ⦄ ∈ ⟦ B ⟧ᵉ
 notation:40 Γ:41 "⊨" v:41 "∶" A:41 => semVal Γ v A
-notation:40 Γ:41 "⊨" m:41 "∶" B:41 => semCom Γ m B
+notation:40 Γ:41 "∣" Δ:41 "⊨" m:41 "∶" B:41 => semCom Γ Δ m B
 
 /-*----------------------------------------
   Fundamental theorem of soundness
@@ -81,7 +95,7 @@ notation:40 Γ:41 "⊨" m:41 "∶" B:41 => semCom Γ m B
 
 theorem soundness {Γ} :
   (∀ (v : Val) A, Γ ⊢ v ∶ A → Γ ⊨ v ∶ A) ∧
-  (∀ (m : Com) B, Γ ⊢ m ∶ B → Γ ⊨ m ∶ B) := by
+  (∀ {Δ} (m : Com) B, Γ ∣ Δ ⊢ m ∶ B → Γ ∣ Δ ⊨ m ∶ B) := by
   refine ⟨λ v A h ↦ ?val, λ m B h ↦ ?com⟩
   mutual_induction h, h
   all_goals intro σ hσ
@@ -89,70 +103,87 @@ theorem soundness {Γ} :
   case unit => exact 𝒱.unit
   case inl ih => exact 𝒱.inl (ih σ hσ)
   case inr ih => exact 𝒱.inr (ih σ hσ)
-  case thunk ih => exact 𝒱.thunk (ih σ hσ)
+  case thunk ih =>
+    let hm := ih σ hσ jid semDtxtNil
+    rw [substJid] at hm; exact 𝒱.thunk hm
+  all_goals intro τ hτ
   case force ih =>
     simp [𝒱, ℰ] at ih
     let ⟨_, ⟨_, ⟨r, _⟩, h⟩, e⟩ := ih σ hσ
     let rf : _ ⇒⋆ _ := .trans .π r
-    rw [← e] at rf
-    exact 𝒞bwd rf h
+    rw [← e] at rf; exact 𝒞bwd rf h
   case lam ih =>
     apply 𝒞ℰ; apply 𝒞.lam
     intro v hv; rw [← substUnion]
-    exact ih (v +: σ) (semCtxtCons hv hσ)
+    let hm := ih (v +: σ) (semCtxtCons hv hσ) jid semDtxtNil
+    rw [substJid] at hm; exact hm
   case app ihm ihv =>
     simp [ℰ, 𝒞] at ihm
-    let ⟨_, ⟨rlam, _⟩, _, h, e⟩ := ihm σ hσ; subst e
+    let ⟨_, ⟨rlam, _⟩, _, h, e⟩ := ihm σ hσ jid semDtxtNil; subst e
     let ⟨_, ⟨rval, _⟩, h⟩ := h _ (ihv σ hσ)
+    rw [substJid] at rlam
     exact 𝒞bwd (Trans.trans (Evals.app rlam) (Trans.trans Eval.β rval)) h
   case ret ih => exact 𝒞ℰ (𝒞.ret (ih σ hσ))
-  case letin ihret ih =>
+  case letin n _ _ _ _ ihret ih =>
     simp [ℰ, 𝒞] at ihret ih
-    let ⟨_, ⟨rret, _⟩, v, hv, e⟩ := ihret σ hσ; subst e
-    let ⟨_, ⟨rlet, nflet⟩, h⟩ := ih (v +: σ) (semCtxtCons hv hσ)
+    let ⟨_, ⟨rret, _⟩, v, hv, e⟩ := ihret σ hσ jid semDtxtNil; subst e
+    let ⟨_, ⟨rlet, nflet⟩, h⟩ := ih (v +: σ) (semCtxtCons hv hσ) _ (semDtxtCons₁ hτ)
     rw [substUnion] at rlet
+    rw [substJid] at rret
     exact 𝒞bwd (Trans.trans (Evals.let rret) (Trans.trans Eval.ζ rlet)) h
   case case m n _ _ _ _ _ _ ihv ihm ihn =>
     simp [𝒱] at ihv
     match ihv σ hσ with
     | .inl ⟨v, hv, e⟩ =>
-      let hm := ihm (v +: σ) (semCtxtCons hv hσ)
-      simp only [substCom]; rw [e]; rw [substUnion] at hm
+      let hm := ihm (v +: σ) (semCtxtCons hv hσ) _ (semDtxtCons₁ hτ)
+      simp [substJoin, substCom]; rw [e]; rw [substUnion] at hm
       exact ℰbwd (.once .ιl) hm
     | .inr ⟨v, hv, e⟩ =>
-      let hn := ihn (v +: σ) (semCtxtCons hv hσ)
-      simp only [substCom]; rw [e]; rw [substUnion] at hn
+      let hn := ihn (v +: σ) (semCtxtCons hv hσ) _ (semDtxtCons₁ hτ)
+      simp [substJoin, substCom]; rw [e]; rw [substUnion] at hn
       exact ℰbwd (.once .ιr) hn
   case prod m n _ _ _ _ ihm ihn =>
     simp [ℰ, 𝒞] at ihm ihn
-    let ⟨_, ⟨rm, _⟩, hm⟩ := ihm σ hσ
-    let ⟨_, ⟨rn, _⟩, hn⟩ := ihn σ hσ
+    let ⟨_, ⟨rm, _⟩, hm⟩ := ihm σ hσ jid semDtxtNil
+    let ⟨_, ⟨rn, _⟩, hn⟩ := ihn σ hσ jid semDtxtNil
+    rw [substJid] at rm rn
     apply 𝒞ℰ; exact 𝒞.prod (𝒞bwd rm hm) (𝒞bwd rn hn)
   case fst ih =>
     simp [ℰ] at ih; unfold 𝒞 at ih
-    let ⟨_, ⟨rprod, nfprod⟩, n₁, n₂, hm, _, e⟩ := ih σ hσ; subst e
+    let ⟨_, ⟨rprod, nfprod⟩, n₁, n₂, hm, _, e⟩ := ih σ hσ jid semDtxtNil; subst e
+    rw [substJid] at rprod
     let r : fst (_⦃σ⦄) ⇒⋆ n₁ := Trans.trans (Evals.fst rprod) Eval.π1
     exact ℰbwd r hm
   case snd ih =>
     simp [ℰ] at ih; unfold 𝒞 at ih
-    let ⟨_, ⟨rprod, nfprod⟩, n₁, n₂, _, hn, e⟩ := ih σ hσ; subst e
+    let ⟨_, ⟨rprod, nfprod⟩, n₁, n₂, _, hn, e⟩ := ih σ hσ jid semDtxtNil; subst e
+    rw [substJid] at rprod
     let r : snd (_⦃σ⦄) ⇒⋆ n₂ := Trans.trans (Evals.snd rprod) Eval.π2
     exact ℰbwd r hn
+  case join Γ Δ m _ A B _ _ ihm ihn =>
+    simp [ℰ] at ihn
+    let hm := λ {σ v} hσ hv ↦ ihm (v +: σ) (semCtxtCons hv hσ) _ (semDtxtCons₁ hτ)
+    let ⟨n, ⟨r, _⟩, hn⟩ := ihn σ hσ _ (semDtxtCons₂ hm hτ)
+    refine 𝒞bwd ?_ hn
+    simp; sorry
+  case jump j v _ _ mem _ ihv =>
+    simp [substJoin, substPush]
+    exact hτ hσ mem (ihv σ hσ)
 
 -- If a computation does not step, then it is in normal form
-theorem normal {m B} (nr : ∀ {n}, ¬ m ⇒ n) (h : ⬝ ⊢ m ∶ B) : nf m := by
+theorem normal {m B} (nr : ∀ {n}, ¬ m ⇒ n) (h : ⬝ ∣ ⬝ ⊢ m ∶ B) : nf m := by
   let ⟨_, soundCom⟩ := soundness (Γ := ⬝)
   let mB := soundCom m B h
   simp [ℰ] at mB
-  let ⟨_, ⟨r, nfm⟩, _⟩ := mB var semCtxtNil
-  rw [substComId] at r
+  let ⟨_, ⟨r, nfm⟩, _⟩ := mB var semCtxtNil jid semDtxtNil
+  rw [substComId, substJid] at r
   cases r with | refl => exact nfm | trans r _ => cases nr r
 
 -- Computations are strongly normalizing
-theorem normalization {m : Com} {B : ComType} (h : ⬝ ⊢ m ∶ B) : SN m := by
+theorem normalization {m : Com} {B : ComType} (h : ⬝ ∣ ⬝ ⊢ m ∶ B) : SN m := by
   let ⟨_, soundCom⟩ := soundness (Γ := ⬝)
   let mB := soundCom m B h
   simp [ℰ] at mB
-  let ⟨_, ⟨r, nfm⟩, _⟩ := mB var semCtxtNil
-  rw [substComId] at r
+  let ⟨_, ⟨r, nfm⟩, _⟩ := mB var semCtxtNil jid semDtxtNil
+  rw [substComId, substJid] at r
   exact r.sn nfm
